execution/tests/FA2Tests/FA2Printers.v
@@ -208,7 +208,7 @@ Instance showFA2Interfaceset_hook_param : Show FA2Interface.set_hook_param :=
 Instance showFA2ReceiverMsg {Msg : Type}
                            `{serMsg : Serializable Msg}
                            `{Show Msg}
-                           : Show (@FA2ReceiverMsg _ Msg serMsg) :=
+                           : Show (@FA2ReceiverMsg _ Msg) :=
 {|
   show m := match m with
             | receive_balance_of_param param => "receive_balance_of_param " ++ show param
@@ -223,7 +223,7 @@ Instance showFA2ReceiverMsg {Msg : Type}
 Instance showFA2TransferHook {Msg : Type}
                             `{serMsg : Serializable Msg}
                             `{Show Msg}
-                             : Show (@FA2TransferHook _ Msg serMsg) :=
+                             : Show (@FA2TransferHook _ Msg) :=
 {|
   show m := match m with
             | transfer_hook param => "transferhook " ++ show param
